---
print_background: true
export_on_save:
    html: true
puppeteer:
    format: "Letter"
    timeout: 3000
    scale: 0.8
---

# Homework 11


## 1. Find the singular value decomposition of the following two matrices.

### (a) $$\begin{bmatrix}1 & -2 \\-3 & 6\end{bmatrix}$$

Let $A=\begin{bmatrix}1 & -2 \\-3 & 6\end{bmatrix}$.

$$
A^\top A=\begin{bmatrix}
    1 & -3 \\ -2 & 6
\end{bmatrix}\begin{bmatrix}
    1 & -2 \\ -3 & 6
\end{bmatrix}
=\begin{bmatrix}
    10 & -20 \\
    -20 & 40
\end{bmatrix} \\
\begin{align*}
    \det(A^\top A-\lambda I)
    &= \begin{bmatrix}
        10-\lambda & -20 \\
        -20 & 40-\lambda
    \end{bmatrix} &= 0 \\
    &= (10-\lambda)(40-\lambda) - (-20)(-20) &= 0 \\
    &= \lambda^2 - 50\lambda &= 0 \\
    &= \lambda(\lambda - 50) &= 0
\end{align*}
\\
\therefore \lambda = 0, 50
$$

$\lambda_1 = 0$ and $\lambda_2=50$ are the eigenvalues of $A^\top A$.

$$
\begin{array}{c}
        \lambda_1 = 0 &\implies &\sigma_1 = 0 \\
        \lambda_2 = 50 &\implies &\sigma_2 = \sqrt{50} = 5\sqrt{2}
    \end{array}
\\[1em]
\boxed{\therefore\Sigma = \begin{bmatrix}
        0 & 0 \\
        0 & 5\sqrt{2}
    \end{bmatrix}
}
$$

And so:

$$
\operatorname{rref}(A^\top A - \lambda_1 I)
= \operatorname{rref} \begin{bmatrix}
    10-0 & -20 \\
    -20 & 40-0
\end{bmatrix}
= \begin{bmatrix}
    1 & -2 \\ 0 & 0
\end{bmatrix}
\\
\therefore \ker(A^\top A - \lambda_1 I)
= \ker\begin{bmatrix}
    1 & -2 \\ 0 & 0
\end{bmatrix}
= \operatorname{span}\Set{
    \begin{bmatrix}
        2 \\ 1
    \end{bmatrix}
}
$$

As such, $\vector{v}_1 = \displaystyle\frac{1}{\sqrt{5}}\begin{bmatrix}
    2 \\ 1
\end{bmatrix}$ is an eigenvector corresponding to $\lambda_1=0$.

$$
\operatorname{rref}(A^\top A - \lambda_2 I)
= \operatorname{rref} \begin{bmatrix}
    10-50 & -20 \\
    -20 & 40-50
\end{bmatrix}
= \begin{bmatrix}
    1 & 1/2 \\ 0 & 0
\end{bmatrix}
\\
\therefore \ker(A^\top A - \lambda_2 I)
= \ker\begin{bmatrix}
    1 & 1/2 \\ 0 & 0
\end{bmatrix}
= \operatorname{span}\Set{
    \begin{bmatrix}
        -1/2 \\ 1
    \end{bmatrix}
}
$$

As such, $\vector{v}_2 = \displaystyle\frac{2}{\sqrt{5}}\begin{bmatrix}
    -1/2 \\ 1
\end{bmatrix}$ is an eigenvector corresponding to $\lambda_2=50$.

$$
\boxed{
    \therefore V = \begin{bmatrix}
        2/\sqrt{5} & -1/\sqrt{5} \\
        1/\sqrt{5} &  2/\sqrt{5}
    \end{bmatrix} = \frac{1}{\sqrt{5}} \begin{bmatrix}
        2 & -1 \\ 1 & 2
    \end{bmatrix}
}
$$


Then, $\vector{u}_i = \displaystyle\frac{1}{\sigma_i}A\vector{v}_i$ for $i=1,2$:

Note $\sigma_1 = 0$, so we move on to $\vector{u}_2$.

$$
\begin{align*}
    \vector{u}_2 &= \frac{1}{5\sqrt{2}}\begin{bmatrix}
        1 & -2 \\
        -3 & 6
    \end{bmatrix}
    \frac{2}{\sqrt{5}}\begin{bmatrix}
        -1/2 \\ 1
    \end{bmatrix} \\
    &= \frac{1}{\sqrt{10}}\begin{bmatrix}
        -1 \\ 3
    \end{bmatrix}
\end{align*}
$$

Since $\sigma_1=0$ and we need one more vector, we need to choose a vector $\vector{u}_1$ such that it is orthogonal to $\vector{u}_2$. Since it's just $\R^2$, we can just eyeball and make $\displaystyle\vector{u}_1 = \frac{1}{\sqrt{10}}\begin{bmatrix}
    3 \\ 1
\end{bmatrix}$.

Sanity check: $\displaystyle\langle\vector{u}_1,\vector{u}_2\rangle = \frac{1}{\sqrt{10}}((-1)(3) + 3(1)) = 0$.

$$
\boxed{
    \therefore U = \begin{bmatrix}
        3/\sqrt{10} & -1/\sqrt{10} \\
        1/\sqrt{10} & 3/\sqrt{10}
    \end{bmatrix} = \frac{1}{\sqrt{10}} \begin{bmatrix}
        3 & -1 \\ 1 & 3
    \end{bmatrix}
}
$$

And so, we have that the SVD for $A=\begin{bmatrix}1 & -2 \\-3 & 6\end{bmatrix}$ is:

$$
\begin{align*}
    A &= U\Sigma V^\top \\
    &= \begin{bmatrix}
        3/\sqrt{10} & -1/\sqrt{10} \\
        1/\sqrt{10} & 3/\sqrt{10}
    \end{bmatrix}\begin{bmatrix}
        0 & 0 \\
        0 & 5\sqrt{2}
    \end{bmatrix}\begin{bmatrix}
        2/\sqrt{5} & -1/\sqrt{5} \\
        1/\sqrt{5} &  2/\sqrt{5}
    \end{bmatrix}^\top \\
    &= \frac{1}{\sqrt{10}}\begin{bmatrix}
        3 & -1 \\
        1 & 3
    \end{bmatrix}\begin{bmatrix}
        0 & 0 \\
        0 & 5\sqrt{2}
    \end{bmatrix}\frac{1}{\sqrt{5}}\begin{bmatrix}
        2 & 1 \\
        -1 & 2
    \end{bmatrix} \\
    &= \begin{bmatrix}
        1 & -2 \\
        -3 & 6
    \end{bmatrix}
\end{align*}
$$

### (b) $$\begin{bmatrix}2 & 1 & 0 & -1 \\0 & -1 & 1 & -1\end{bmatrix}$$

Let $A=\begin{bmatrix}2 & 1 & 0 & -1 \\0 & -1 & 1 & -1\end{bmatrix}$.

$$
A^\top A = \begin{bmatrix}
    4 & 2 & 0 & -2 \\
    2 & 2 & -1 & 0 \\
    0 & -1 & 1 & -1 \\
    -2 & 0 & -1 & 2
\end{bmatrix} \\
\begin{align*}
    \det(A^\top A-\lambda I)
    &= \begin{bmatrix}
        4-\lambda & 2 & 0 & -2 \\
        2 & 2-\lambda & -1 & 0 \\
        0 & -1 & 1-\lambda & -1 \\
        -2 & 0 & -1 & 2-\lambda
    \end{bmatrix} &= 0 \\
    &= \lambda^4 - 9\lambda^3 + 18\lambda^2 &= 0 \\
    &= \lambda^2(\lambda - 3)(\lambda - 6) &= 0
\end{align*}
\\
\therefore \lambda = 0,3,6
$$

$\lambda_1=0$, $\lambda_2=3$, and $\lambda_3=6$ are eigenvalues of $A^\top A$.

$$
\begin{array}{c}
    \lambda_1 = 0 &\implies &\sigma_1 = 0 \\
    \lambda_2 = 3 &\implies &\sigma_2 = \sqrt{3} \\
    \lambda_3 = 6 &\implies &\sigma_3 = \sqrt{6}
\end{array}
\\[1em]
\boxed{
    \therefore\Sigma = \begin{bmatrix}
        \sqrt{3} & 0 & 0 & 0 \\
        0 & \sqrt{6} & 0 & 0
    \end{bmatrix}
}
$$

And so:

$$
\operatorname{rref}(A^\top A - \lambda_1 I)
= \operatorname{rref} \begin{bmatrix}
        4-0 & 2 & 0 & -2 \\
        2 & 2-0 & -1 & 0 \\
        0 & -1 & 1-0 & -1 \\
        -2 & 0 & -1 & 2-0
    \end{bmatrix}
= \begin{bmatrix}
        1 & 0 & 1/2 & -1 \\
        0 & 1 & -1 & 1 \\
        0 & 0 & 0 & 0 \\
        0 & 0 & 0 & 0
    \end{bmatrix}
\\
\therefore \ker(A^\top A - \lambda_1 I)
= \ker\begin{bmatrix}
        1 & 0 & 1/2 & -1 \\
        0 & 1 & -1 & 1 \\
        0 & 0 & 0 & 0 \\
        0 & 0 & 0 & 0
    \end{bmatrix}
= \operatorname{span}\Set{
    \begin{bmatrix}
        -1/2 \\ 1 \\ 1 \\ 0
    \end{bmatrix},
    \begin{bmatrix}
        1 \\ -1 \\ 0 \\ 1
    \end{bmatrix}
}
$$

As such, $\displaystyle\frac{2}{3}\begin{bmatrix}
        -1/2 \\ 1 \\ 1 \\ 0
    \end{bmatrix},\frac{1}{\sqrt{3}}
    \begin{bmatrix}
        1 \\ -1 \\ 0 \\ 1
\end{bmatrix}$ are eigenvectors corresponding to $\lambda_1=0$.

$$
\operatorname{rref}(A^\top A - \lambda_2 I)
= \operatorname{rref} \begin{bmatrix}
        4-3 & 2 & 0 & -2 \\
        2 & 2-3 & -1 & 0 \\
        0 & -1 & 1-3 & -1 \\
        -2 & 0 & -1 & 2-3
    \end{bmatrix}
= \begin{bmatrix}
        1 & 0 & 0 & 0 \\
        0 & 1 & 0 & -1 \\
        0 & 0 & 1 & 1 \\
        0 & 0 & 0 & 0
    \end{bmatrix}
\\
\therefore \ker(A^\top A - \lambda_2 I)
= \ker\begin{bmatrix}
        1 & 0 & 0 & 0 \\
        0 & 1 & 0 & -1 \\
        0 & 0 & 1 & 1 \\
        0 & 0 & 0 & 0
    \end{bmatrix}
= \operatorname{span}\Set{
    \begin{bmatrix}
        0 \\ 1 \\ -1 \\ 1
    \end{bmatrix}
}
$$

As such, $\vector{v}_2 = \displaystyle\frac{1}{\sqrt{3}}\begin{bmatrix}
    0 \\ 1 \\ -1 \\ 1
\end{bmatrix}$ is an eigenvector corresponding to $\lambda_2=3$.


$$
\operatorname{rref}(A^\top A - \lambda_3 I)
= \operatorname{rref} \begin{bmatrix}
        4-6& 2 & 0 & -2 \\
        2 & 2-6& -1 & 0 \\
        0 & -1 & 1-6& -1 \\
        -2 & 0 & -1 & 2-6    \end{bmatrix}
= \begin{bmatrix}
    1 & 0 & 0 & 2 \\
    0 & 1 & 0 & 1 \\
    0 & 0 & 1 & 0 \\
    0 & 0 & 0 & 0
\end{bmatrix}
\\
\therefore \ker(A^\top A - \lambda_3 I)
= \ker\begin{bmatrix}
    1 & 0 & 0 & 2 \\
    0 & 1 & 0 & 1 \\
    0 & 0 & 1 & 0 \\
    0 & 0 & 0 & 0
\end{bmatrix}
= \operatorname{span}\Set{
    \begin{bmatrix}
        -2 \\ -1 \\ 0 \\ 1
    \end{bmatrix}
}
$$

As such, $\vector{v}_3 = \displaystyle\frac{1}{\sqrt{6}} \begin{bmatrix}
    -2 \\ -1 \\ 0 \\ 1
\end{bmatrix}$ is an eigenvector corresponding to $\lambda_3=6$.

$$
\boxed{
    \therefore V = \begin{bmatrix}
       -1/3 & 1/\sqrt{3} & 0 &-\sqrt{2/3} \\
       2/3 & -1/\sqrt{3} & 1/\sqrt{3} & -1/\sqrt{6} \\
       2/3 & 0 & -1/\sqrt{3} & 0 \\
       0 & 1/\sqrt{3} & 1/\sqrt{3} & 1/\sqrt{6}
    \end{bmatrix}
}\\ \;
$$

Then, $\vector{u}_i = \displaystyle\frac{1}{\sigma_i}A\vector{v}_i$ for $i=2,3$:

$$
\begin{align*}
    \vector{u}_2 &= \frac{1}{\sqrt{3}}\begin{bmatrix}
        2 & 1 & 0 & -1 \\
        0 & -1 & 1 & -1
    \end{bmatrix}
    \frac{1}{\sqrt{3}}\begin{bmatrix}
        0 \\ 1 \\ -1 \\ 1
    \end{bmatrix} \\
    &= \begin{bmatrix}
        0 \\ -1
    \end{bmatrix} \\
    \vector{u}_3 &= \frac{1}{\sqrt{6}}\begin{bmatrix}
        2 & 1 & 0 & -1 \\
        0 & -1 & 1 & -1
        \end{bmatrix}\frac{1}{\sqrt{6}} \begin{bmatrix}
        -2 \\ -1 \\ 0 \\ 1
    \end{bmatrix} \\
    &= \begin{bmatrix}
        -1 \\ 0
    \end{bmatrix}
\end{align*}
\\[1em]
\boxed{
    \therefore U = \begin{bmatrix}
        0 & -1 \\ -1 & 0
    \end{bmatrix}
}
$$

And so, we have that the SVD for $A=\begin{bmatrix}1 & -2 \\-3 & 6\end{bmatrix}$ is:

$$
\begin{align*}
    A &= U\Sigma V^\top \\
    &= \begin{bmatrix}
        0 & -1 \\ -1 & 0
    \end{bmatrix}
    \begin{bmatrix}
        \sqrt{3} & 0 & 0 & 0 \\
        0 & \sqrt{6} & 0 & 0
    \end{bmatrix}
    \begin{bmatrix}
       -1/3 & 1/\sqrt{3} & 0 &-\sqrt{2/3} \\
       2/3 & -1/\sqrt{3} & 1/\sqrt{3} & -1/\sqrt{6} \\
       2/3 & 0 & -1/\sqrt{3} & 0 \\
       0 & 1/\sqrt{3} & 1/\sqrt{3} & 1/\sqrt{6}
    \end{bmatrix}^\top \\
    &= \begin{bmatrix}
        0 & -1 \\ -1 & 0
    \end{bmatrix}
    \begin{bmatrix}
        \sqrt{3} & 0 & 0 & 0 \\
        0 & \sqrt{6} & 0 & 0
    \end{bmatrix}
    \begin{bmatrix}
        -1/3 & 2/3 & 2/3 & 0 \\
        1/\sqrt{3} & -1/\sqrt{3} & 0 & 1/\sqrt{3} \\
        0 & 1/\sqrt{3} & -1/\sqrt{3} & 1/\sqrt{3} \\
        -\sqrt{2/3} & -1/\sqrt{6} & 0 & 1/\sqrt{6}
    \end{bmatrix} \\
    &= \begin{bmatrix}
        2 & 1 & 0 & -1 \\
        0 & -1 & 1 & -1
    \end{bmatrix}
\end{align*}
$$


## 2. A famous application of spectral theorem and SVD is the spectral graph theory. A graph $(V, E)$ is a set of vertices $V$ with edge set $E$. We say that for $x, y \in V , x \sim y$ if $x$ and $y$ are connected by an edge in $E$. The **Graph Laplacian** is defined to be a matrix $A$ of size $|V|\times|V|$

$$
A_{x,y} = \begin{cases}
1 & \text{if $x \sim y$} \\
-\text{(number of edges starting from $x$)} & \text{if $x = y$} \\
0 & \text{otherwise}
\end{cases}
$$

For example, a triangle with three vertices

$$
A = \begin{bmatrix}
    -2 & 1 & 1 \\
    1 & -2 & 1 \\
    1 & 1 & -2
\end{bmatrix}
$$

### (a) Find the SVD for the Laplacian of the triangle graph.

Using an online calculator, we find $A = U\Sigma V^\top$ for

$$
U = \begin{bmatrix}
    1/\sqrt{2} & 1/\sqrt{6} & 1/\sqrt{3} \\
    0 & -\sqrt{2/3} & 1/\sqrt{3} \\
    -1/\sqrt{2} & 1/\sqrt{6} & 1/\sqrt{3}
\end{bmatrix},\quad
\Sigma = \begin{bmatrix}
    3 & 0 & 0 \\
    0 & 3 & 0 \\
    0 & 0 & 0
\end{bmatrix},\quad
V = \begin{bmatrix}
    -1/\sqrt{2} & -1/\sqrt{6} & 1/\sqrt{3} \\
    0 & \sqrt{2/3} & 1/\sqrt{3} \\
    1/\sqrt{2} & -1/\sqrt{6} & 1/\sqrt{3}
\end{bmatrix}.
$$

### (b) Write down the graph Laplacian matrix for the square graph and then find its SVD.


Using the definition above, the Laplacian matrix $A$ for a square graph is:

$$
A = \begin{bmatrix}
    2 & -1 & 0 & -1 \\
    -1 & 2 & -1 & 0 \\
    0 & -1 & 2 & -1 \\
    -1 & 0 & -1 & 2
\end{bmatrix}
$$

Again, sparing the computation. The SVD for the square graph $A = U\Sigma V^\top$ is given by:

$$
U = V = \begin{bmatrix}
-1/2 & 0 & -1/\sqrt{2} & 1/2 \\
1/2 & -1/\sqrt{2} & 0 & 1/2 \\
-1/2 & 0 & 1/\sqrt{2} & 1/2 \\
1/2 & 1/\sqrt{2} & 0 & 1/2
\end{bmatrix},\quad
\Sigma = \begin{bmatrix}
4 & 0 & 0 & 0 \\
0 & 2 & 0 & 0 \\
0 & 0 & 2 & 0 \\
0 & 0 & 0 & 0
\end{bmatrix}
$$




